\documentclass{article}

\begin{document}

  \textbf{Problem:} Given A, B, and n. Find :
  $$
    \sum_{i = 0}^{n} F_{A + i} F_{B + i}
  $$

  \begin{equation}
    k = A - B
  \end{equation}


  \begin{equation}
    F_{A} F_{B} = F_{k + 1} F_{A} ^ 2 + F_{k} F_{A} F_{A - 1}
  \end{equation}

  \begin{equation}
    \sum_{i = 0}^{n} F_{i} ^ 2 = F_{n + 1} F_{n}
  \end{equation}

  $ev(n)$ = returns 1 if $n$ is even.

  \begin{equation}
    \sum_{i = 0}^{n} F_{i} F_{i + 1} = F_{n + 1} ^ {2} - ev(n)
  \end{equation}

  \begin{equation}
    \sum_{i = 0}^{n} F_{i} F_{i - 1} = \sum_{i = 0}^{n - 1} F_{i} F_{i + 1}
  \end{equation}


  \begin{equation}
    \sum_{i = 0}^{n} F_{A + i} F_{B + i} =  \sum_{i = 0}^{n} F_{k + 1} F_{A + i}^{2}
    +  \sum_{i = 0}^{n} F_{k} F_{A + i} F_{A + i - 1}
  \end{equation}

  \begin{equation}
    \sum_{i = 0}^{n} F_{A + i} F_{B + i} =  F_{k + 1} \sum_{i = 0}^{n} F_{A + i}^{2}
    +  F_{k} \sum_{i = 0}^{n} F_{A + i} F_{A + i - 1}
  \end{equation}

  \begin{equation}
    \sum_{i = 0}^{n} F_{A + i} F_{B + i} =  F_{k + 1} F_{A + n - 1} F_{A + n}
    - F_{k - 1} F_{A - 1} F_{A}
    +  F_{k} \sum_{i = 0}^{n} F_{A + i} F_{A + i - 1}
  \end{equation}

  \begin{equation}
    \sum_{i = 0}^{n} F_{A + i} F_{B + i} =  F_{k + 1} F_{A + n - 1} F_{A + n}
    - F_{k - 1} F_{A - 1} F_{A}
    + F_{A + n - 2} ^ {2} - ev(A + n - 2)
    + F_{A + - 2} ^ {2} - ev(A - 2)
  \end{equation}

\end{document}
